STLC_SuccNat/Lifted_Msubst.v
@@ -1,0 +1,222 @@
+Require Import String List Maps.
+Import ListNotations.
+Require Import STLC_SuccNat.
+Require Import Lifted_STLC_SuccNat.
+Require Import Environments.
+
+Hint Constructors multi : core.
+Hint Constructors value' : core.
+Hint Constructors step' : core.
+Hint Constructors has_type' : core.
+
+Hint Extern 2 (has_type' _ (app' _ _) _) => eapply T_App'; auto : core.
+Hint Extern 2 (_ = _) => compute; reflexivity : core.
+
+Definition halts' t' : Prop := exists t1', multi step' t' t1' /\ value' t1'.
+
+Lemma value'_halts' : forall v', value' v' -> halts' v'.
+Proof.
+  intros v H. unfold halts'.
+  exists v. split.
+  - apply multi_refl.
+  - assumption.
+Qed.
+
+Inductive appears_free_in' : string -> tm' -> Prop :=
+  |afi_var' : forall (x:string), appears_free_in' x (var' x)
+  |afi_app1' : forall x t1' t2',
+    appears_free_in' x t1' -> appears_free_in' x (app' t1' t2')
+  |afi_app2' : forall x t1' t2',
+    appears_free_in' x t2' -> appears_free_in' x (app' t1' t2')
+  |afi_abs' : forall x y T11' t12',
+    y <> x -> appears_free_in' x t12' ->
+      appears_free_in' x (abs' y T11' t12')
+  |afi_fixp' : forall x t1',
+    appears_free_in' x t1' ->
+      appears_free_in' x (fixp' t1')
+  (* nats*)
+  |afi_succ' : forall x t1', appears_free_in' x t1' -> appears_free_in' x (succ' t1').
+
+Hint Constructors appears_free_in' : core.
+
+Definition closed' (t':tm') :=
+  forall x, ~ appears_free_in' x t'.
+
+Lemma context'_invariance: forall Gamma' Gamma1' t' S',
+  has_type' Gamma' t' S' ->
+  (forall x, appears_free_in' x t' -> Gamma' x = Gamma1' x) ->
+  has_type' Gamma1' t' S'.
+Proof.
+  intros.
+  generalize dependent Gamma1'.
+  induction H; intros; eauto 12.
+  - (* T_Var' *)
+    apply T_Var'. rewrite <- H0; auto.
+  - (* T_Abs' *)
+    apply T_Abs'.
+    apply IHhas_type'. intros x1 Hafi.
+    (* the only tricky step... *)
+    destruct (eqb_spec x x1); subst.
+    + rewrite update_eq.
+      rewrite update_eq.
+      reflexivity.
+    + rewrite update_neq; [| assumption].
+      rewrite update_neq; [| assumption].
+      auto.
+Qed.
+
+Theorem false_eqb_string : forall x y : string,
+   x <> y -> String.eqb x y = false.
+Proof.
+  intros x y. rewrite String.eqb_neq.
+  intros H. apply H. Qed.
+
+Lemma free_in_context' : forall x t' T' Gamma',
+   appears_free_in' x t' ->
+   has_type' Gamma' t' T' ->
+   exists T1', Gamma' x = Some T1'.
+Proof with eauto.
+  intros x t T Gamma Hafi Htyp.
+  induction Htyp; inversion Hafi; subst...
+  - (* T_Abs' *)
+    destruct IHHtyp as [T' Hctx]... exists T'.
+    unfold update, t_update in Hctx.
+    rewrite false_eqb_string in Hctx...
+Qed.
+
+Corollary typable_empty__closed' : forall t' T',
+    has_type' empty t' T'  -> closed' t'.
+Proof.
+  intros. unfold closed'. intros x H1.
+  destruct (free_in_context' _ _ _ _ H1 H) as [T1' C].
+  discriminate C.
+Qed.
+
+Lemma vacuous_substitution' : forall  t' x,
+     ~ appears_free_in' x t'  ->
+     forall t1', subst' x t1' t' = t'.
+Proof with eauto.
+  induction t'; intros x Hnafi t1';
+    simpl; eauto.
+  - (* Var' *)
+    rename s into y. destruct (eqb_spec x y); simpl.
+    exfalso. subst...
+    reflexivity.
+  - (* Abs' *)
+    rename s into y. destruct (eqb_spec x y); simpl.
+    reflexivity.
+    f_equal. apply IHt'.
+    intros H. apply Hnafi.
+    apply afi_abs'...
+ - (* App' *)
+    rewrite IHt'1, IHt'2.
+    reflexivity.
+    intros H; eauto.
+    intros H; eauto.
+ - (* Fixp' *)
+    rewrite IHt'...
+ - (* Succ' *)
+    rewrite IHt'...
+Qed.
+
+Lemma subst'_closed': forall t',
+  closed' t' -> forall x t1', subst' x t1' t' = t'.
+Proof.
+  intros. apply vacuous_substitution'. apply H.
+Qed.
+
+Lemma msubst'_closed': forall t', closed' t' -> forall ss, msubst' ss t' = t'.
+Proof.
+  induction ss.
+    reflexivity.
+    destruct a. simpl. rewrite subst'_closed'; assumption.
+Qed.
+
+Fixpoint closed'_env' (env':env') :=
+  match env' with
+  | nil => True
+  | (x,t')::env1' => closed' t' /\ closed'_env' env1'
+  end.
+
+Lemma subst'_not_afi' : forall t' x v',
+    closed' v' ->  ~ appears_free_in' x (subst' x v' t').
+Proof with eauto.  (* rather slow this way *)
+  unfold closed', not.
+  induction t'; intros x v P A; simpl in A.
+    - (* var' *)
+     destruct (eqb_spec x s)...
+     inversion A; subst. auto.
+    - (* abs' *)
+     destruct (eqb_spec x s)...
+     + inversion A; subst...
+     + inversion A; subst...
+    - (* app' *)
+     inversion A; subst...
+    - (* fixp' *)
+     inversion A; subst...
+    - (* const' *)
+     inversion A.
+    - (* succ' *)
+     inversion A; subst...
+Qed.
+
+Lemma duplicate_subst' : forall t1' x t' v',
+  closed' v' -> (subst' x t' (subst' x v' t1')) = (subst' x v' t1').
+Proof.
+  intros. eapply vacuous_substitution'. apply subst'_not_afi'. assumption.
+Qed.
+
+Lemma swap_subst' : forall t' x x1 v' v1',
+    x <> x1 ->
+    closed' v' -> closed' v1' ->
+    (subst' x1 v1' (subst' x v' t')) = (subst' x v'(subst' x1 v1' t')).
+Proof with eauto.
+ induction t'; intros; simpl.
+  - (* var' *)
+   destruct (eqb_spec x s); destruct (eqb_spec x1 s).
+   + subst. exfalso...
+   + subst. simpl. rewrite String.eqb_refl. apply subst'_closed'...
+   + subst. simpl. rewrite String.eqb_refl. rewrite subst'_closed'...
+   + simpl. rewrite false_eqb_string... rewrite false_eqb_string...
+  - (* abs' *)
+   destruct (eqb_spec x s); destruct (eqb_spec x1 s).
+   + subst. exfalso...
+   + subst. simpl. rewrite eqb_refl. rewrite false_eqb_string...
+   + subst. simpl. rewrite eqb_refl. rewrite false_eqb_string...
+   + simpl. rewrite false_eqb_string... rewrite false_eqb_string...
+     rewrite IHt'...
+  - (* app' *)
+   rewrite IHt'1, IHt'2...
+  - (* fixp' *)
+   rewrite IHt'...
+  - (* const' *)
+   reflexivity.
+  - (* succ' *)
+   rewrite IHt'...
+Qed.
+
+Lemma subst'_msubst': forall env' x v' t', closed' v' -> closed'_env' env' ->
+    msubst' env' (subst' x v' t') = subst' x v' (msubst' (drop x env') t') .
+Proof.
+  induction env'; intros; auto.
+  destruct a. simpl.
+  inversion H0.
+  destruct (eqb_spec s x).
+  - subst. rewrite duplicate_subst'; auto.
+  - simpl. rewrite swap_subst'; eauto.
+Qed.
+
+Lemma msubst'_var': forall ss x, closed'_env' ss ->
+  msubst' ss (var' x) =
+  match lookup x ss with
+  | Some t' => t'
+  | None => var' x
+  end.
+Proof.
+  induction ss; intros.
+    reflexivity.
+    destruct a.
+      simpl. destruct (eqb s x).
+        apply msubst'_closed'. inversion H; auto.
+        apply IHss. inversion H; auto.
+Qed.
